s2.lock

pulse/share/pulse/examples/PulseCorePaper.S2.Lock.fst
@@ -21,6 +21,15 @@ module Box = Pulse.Lib.Box
 // let storable = is_big
 // let sprop = s:slprop { storable s }
 
+module B = Pulse.Lib.Box
+assume
+val cas_box_alt (r:B.box U32.t) (u v:U32.t) (#i:erased U32.t)
+  : stt_atomic bool #Observable emp_inames 
+    (B.pts_to r i)
+    (fun b ->
+      if b then (B.pts_to r v ** pure (reveal i == u)) 
+           else (B.pts_to r i))
+
 noeq
 type lock = { r:Pulse.Lib.Box.box U32.t; i:iname }
 [@@pulse_unfold]
@@ -31,6 +40,19 @@ let lock_inv r p : v:slprop { is_slprop2 p ==> is_slprop2 v } = exists* v. Box.p
 let protects l p = inv l.i (lock_inv l.r p)
 
 ```pulse
+atomic
+fn mk_lock (r:Box.box U32.t) (i:iname) #p
+requires inv i (lock_inv r p)
+returns l:lock
+ensures protects l p
+{
+  let res = {r;i};
+  rewrite each r as res.r, i as res.i; (* proof hint *)
+  res
+}
+```
+
+```pulse
 fn create (p:storable)
 requires p
 returns l:lock
@@ -38,9 +60,7 @@ ensures protects l p
 {
    let r = Box.alloc 0ul; 
    let i = new_invariant (lock_inv r p);
-   let l = {r;i};
-   rewrite each r as l.r, i as l.i; (* proof hint *)
-   l
+   mk_lock r i
 }
 ```
 
@@ -49,41 +69,26 @@ fn release (#p:slprop) (l:lock)
 requires protects l p ** p
 ensures protects l p
 {
-  unfold protects;
   with_invariants l.i
-    returns _ : unit
-    ensures lock_inv l.r p
-    opens [l.i]
   { 
     drop_ (maybe _ _);
     Pulse.Lib.Primitives.write_atomic_box l.r 0ul;
-  };
-  fold protects;
+  }
 }
 ```
-module B = Pulse.Lib.Box
-assume
-val cas_box_alt (r:B.box U32.t) (u v:U32.t) (#i:erased U32.t)
-  : stt_atomic bool #Observable emp_inames 
-    (B.pts_to r i)
-    (fun b ->
-      if b then (B.pts_to r v ** pure (reveal i == u)) 
-           else (B.pts_to r i))
 
 ```pulse
 fn rec acquire #p (l:lock)
 requires protects l p
 ensures protects l p ** p
 {
-  unfold protects;
-  let b = with_invariants l.i
-    returns b:bool 
-    ensures lock_inv l.r p ** maybe b p
+  let retry = with_invariants l.i
+    returns retry:bool 
+    ensures lock_inv l.r p ** (if retry then emp else p)
   {
     let b = cas_box_alt l.r 0ul 1ul;
-    if b { true } else { false }
+    if b { false } else { true }
   };
-  fold protects;
-  if b { () } else { acquire l }
+  if retry { acquire l }
 }
 ```
